test(TestModels): Extendable-Resources Wrapped in .NET
The following all pass:
```
make polymorph_dafny \
  polymorph_net transpile_net setup_net format_net test_net
```

TestModels/extendable/runtimes/net/Extern/NativeResource.cs
@@ -4,6 +4,7 @@
 using Dafny.Simple.Extendable.Resources;
 using Dafny.Simple.Extendable.Resources.Types;
 using Simple.Extendable.Resources;
+using TypeConversion = Simple.Extendable.Resources.TypeConversion;
 
 namespace Simple.Extendable.Resources
 {
