TestModels/extendable/test/Helpers.dfy
@@ -4,6 +4,7 @@
 include "../src/Index.dfy"
 
 module TestHelpers {
+  import ExtendableResource
   import Types = SimpleExtendableResourcesTypes
   import opened Wrappers
 
@@ -51,6 +52,96 @@ module TestHelpers {
     expect Option.Some(1) == output.longValue; 
   }
 
+  method CheckModeledError(
+    errorOutput: Result<Types.GetExtendableResourceErrorsOutput, Types.Error>
+  )
+  {
+    expect errorOutput.Failure?;
+    var actualError := errorOutput.PropagateFailure<Types.GetExtendableResourceErrorsOutput>().error;
+    expect actualError == Types.SimpleExtendableResourcesException(
+      message := "Hard Coded Exception in src/dafny"
+    );
+  }
+
+  method CheckMultipleErrors(
+    errorOutput: Result<Types.GetExtendableResourceErrorsOutput, Types.Error>
+  )
+  {
+    expect errorOutput.Failure?;
+    var actualError := errorOutput.PropagateFailure<Types.GetExtendableResourceErrorsOutput>().error;
+    // TypeConversion.FromDafny_CommonError does not handle Collection.
+    // As such, even though AlwaysMutlipleErrors correctly returns a Collection in Dafny,
+    // the generated .NET code botches the conversion,
+    // and lumps it as an Opaue Exception.
+    // TODO:
+    // Once https://github.com/awslabs/polymorph/pull/136 is resolved/merged
+    // and smithy-dotnet handles Collections, replace
+    // expect actualError.Opaque? with commented out expect,
+    // and remove this comment.
+    expect actualError.Opaque?;
+    // expect actualError.Collection?
+    //   && |actualError.list| == 1
+    //   && actualError.list[0].SimpleExtendableResourcesException?
+    //   && actualError.list[0].message == "Hard Coded Modeled Exception in Collection";
+  }
+
+  method CheckDafnyMultipleErrors(
+    errorOutput: Result<Types.GetExtendableResourceErrorsOutput, Types.Error>
+  )
+  {
+    expect errorOutput.Failure?;
+    var actualError := errorOutput.PropagateFailure<Types.GetExtendableResourceErrorsOutput>().error;
+    // TypeConversion.FromDafny_CommonError does not handle Collection.
+    // As such, even though AlwaysMutlipleErrors correctly returns a Collection in Dafny,
+    // the generated .NET code botches the conversion,
+    // and lumps it as an Opaue Exception.
+    // TODO:
+    // Once https://github.com/awslabs/polymorph/pull/136 is resolved/merged
+    // and smithy-dotnet handles Collections, replace
+    // expect actualError.Opaque? with commented out expect,
+    // and remove this comment.
+    // expect actualError.Opaque?;
+    expect actualError.Collection?
+      && |actualError.list| == 1
+      && actualError.list[0].SimpleExtendableResourcesException?
+      && actualError.list[0].message == "Hard Coded Modeled Exception in Collection";
+  }
+  
+  method CheckOpaqueError(
+    errorOutput: Result<Types.GetExtendableResourceErrorsOutput, Types.Error>
+  )
+  {
+    expect errorOutput.Failure?;
+    var actualError := errorOutput.PropagateFailure<Types.GetExtendableResourceErrorsOutput>().error;
+    expect actualError.Opaque?
+      // Opaque Errors SHOULD NOT be thrown by Dafny source.
+      // (At least) Smithy-dotnet expects the obj
+      // to be an Exception that it can throw.
+      // It is a PITA to write a class in Dafny
+      // that maps to an Exception in every runtime,
+      // so we are NOT going to do that.
+      // Therefore, we cannot constrain/test the value of obj
+      // with pure Dafny.
+      && !(actualError.obj is ExtendableResource.OpaqueMessage);
+      // For the curious,
+      // in .NET, the obj will be a Native OpaqueError,
+      // with the message:
+      // "Opaque obj is not an Exception."
+      // But we cannot test that here,
+      // as we cannot call the TypeConversion method
+      // from inside Dafny.
+  }
+
+  method CheckDafnyOpaqueError(
+    errorOutput: Result<Types.GetExtendableResourceErrorsOutput, Types.Error>
+  )
+  {
+    expect errorOutput.Failure?;
+    var actualError := errorOutput.PropagateFailure<Types.GetExtendableResourceErrorsOutput>().error;
+    expect actualError.Opaque?
+      && (actualError.obj is ExtendableResource.OpaqueMessage);
+  }
+  
   method {:extern "Simple.Extendable.Resources.NativeResource", "DafnyFactory"} DafnyFactory(
   ) returns (
     output: Types.IExtendableResource
