TestModels/extendable/test/NativeExtendableResourceTest.dfy
@@ -12,9 +12,35 @@ module NativeExtendableResourceTest {
   method {:test} TestNativeResource()
   {
     var resource: Types.IExtendableResource := DafnyFactory();
+    TestSomeGetResourceData(resource);
+    TestNoneGetResourceData(resource);
     TestAlwaysModeledError(resource);
     TestAlwaysMultipleErrors(resource);
     TestAlwaysOpaqueError(resource);
+  }
+
+  method TestSomeGetResourceData(
+    resource: Types.IExtendableResource
+  )
+    requires resource.ValidState()
+    modifies resource.Modifies
+    ensures resource.ValidState()
+  {
+    var dataInput: Types.GetResourceDataInput := allSome();
+    var dataOutput: Types.GetResourceDataOutput :- expect resource.GetResourceData(dataInput);
+    checkSome(dataOutput);
+  }
+
+  method TestNoneGetResourceData(
+    resource: Types.IExtendableResource
+  )
+    requires resource.ValidState()
+    modifies resource.Modifies
+    ensures resource.ValidState()
+  {
+    var dataInput: Types.GetResourceDataInput := allNone();
+    var dataOutput: Types.GetResourceDataOutput :- expect resource.GetResourceData(dataInput);
+    checkNone(dataOutput);
   }
 
   method TestAlwaysModeledError(
@@ -29,11 +55,9 @@ module NativeExtendableResourceTest {
     );
     var errorOutput: Result<Types.GetExtendableResourceErrorsOutput, Types.Error>;
     errorOutput := resource.AlwaysModeledError(errorInput);
-    expect errorOutput.Failure?;
-    var actualError := errorOutput.PropagateFailure<Types.GetExtendableResourceErrorsOutput>().error;
-    expect actualError == Types.SimpleExtendableResourcesException(message := "Hard Coded Exception in src/dafny");
+    CheckModeledError(errorOutput);
   }
-
+  
   method TestAlwaysMultipleErrors(
     resource: Types.IExtendableResource
   )
@@ -46,22 +70,7 @@ module NativeExtendableResourceTest {
     );
     var errorOutput: Result<Types.GetExtendableResourceErrorsOutput, Types.Error>;
     errorOutput := resource.AlwaysMultipleErrors(errorInput);
-    expect errorOutput.Failure?;
-    var actualError := errorOutput.PropagateFailure<Types.GetExtendableResourceErrorsOutput>().error;
-    // TypeConversion.FromDafny_CommonError does not handle Collection.
-    // As such, even though AlwaysMutlipleErrors correctly returns a Collection in Dafny,
-    // the generated .NET code botches the conversion,
-    // and lumps it as an Opaue Exception.
-    // TODO:
-    // Once https://github.com/awslabs/polymorph/pull/136 is resolved/merged
-    // and smithy-dotnet handles Collections, replace
-    // expect actualError.Opaque? with commented out expect,
-    // and remove this comment.
-    expect actualError.Opaque?;
-    // expect actualError.Collection?
-    //   && |actualError.list| == 1
-    //   && actualError.list[0].SimpleExtendableResourcesException?
-    //   && actualError.list[0].message == "Hard Coded Modeled Exception in Collection";
+    CheckMultipleErrors(errorOutput);
   }
 
   method TestAlwaysOpaqueError(
@@ -76,24 +85,6 @@ module NativeExtendableResourceTest {
     );
     var errorOutput: Result<Types.GetExtendableResourceErrorsOutput, Types.Error>;
     errorOutput := resource.AlwaysOpaqueError(errorInput);
-    expect errorOutput.Failure?;
-    var actualError := errorOutput.PropagateFailure<Types.GetExtendableResourceErrorsOutput>().error;
-    expect actualError.Opaque?
-      // Opaque Errors SHOULD NOT be thrown by Dafny source.
-      // (At least) Smithy-dotnet expects the obj
-      // to be an Exception that it can throw.
-      // It is a PITA to write a class in Dafny
-      // that maps to an Exception in every runtime,
-      // so we are NOT going to do that.
-      // Therefore, we cannot constrain/test the value of obj
-      // with pure Dafny.
-      && !(actualError.obj is ExtendableResource.OpaqueMessage);
-      // For the curious,
-      // in .NET, the obj will be a Native OpaqueError,
-      // with the message:
-      // "Opaque obj is not an Exception."
-      // But we cannot test that here,
-      // as we cannot call the TypeConversion method
-      // from inside Dafny.
+    CheckOpaqueError(errorOutput);
   }
 }  
